src3.0/Vellvm/Dominators/dom_type.v
@@ -19,16 +19,20 @@ Import LLVMinfra.
 
 Module Type ALGDOM.
 
-Parameter dom_analysis_is_successful : fdef -> Prop.
-
 Parameter dom_query : fdef -> atom -> set atom.
 
 Axiom dom_entrypoint : forall f l0 ps cs tmn
   (Hentry : getEntryBlock f = Some (block_intro l0 ps cs tmn)),
   dom_query f l0 = nil.
 
-Axiom entry_doms_others: forall (f:fdef) entry
-  (Hex: dom_analysis_is_successful f)
+Definition branchs_in_fdef f :=
+  forall (p : l) (ps0 : phinodes) (cs0 : cmds) 
+         (tmn0 : terminator) (l2 : l),
+  blockInFdefB (block_intro p ps0 cs0 tmn0) f ->
+  In l2 (successors_terminator tmn0) -> In l2 (bound_fdef f).
+
+Axiom entry_doms_others: forall (f:fdef) 
+  (Hbinf: branchs_in_fdef f) (Huniq: uniqFdef f) entry
   (H: getEntryLabel f = Some entry),
   (forall b (H0: b <> entry /\ reachable f b),
      ListSet.set_In entry (dom_query f b)).
@@ -45,29 +49,22 @@ Axiom dom_successors : forall
   incl contents' (l3 :: contents3).
 
 Axiom sdom_is_complete: forall (f:fdef)
+  (Hbinf: branchs_in_fdef f) 
   (l3 : l) (l' : l) ps cs tmn ps' cs' tmn'
   (HuniqF : uniqFdef f)
-  (Hsucc: dom_analysis_is_successful f)
   (HBinF' : blockInFdefB (block_intro l' ps' cs' tmn') f = true)
   (HBinF : blockInFdefB (block_intro l3 ps cs tmn) f = true)
   (Hsdom: strict_domination f l' l3),
   In l' (dom_query f l3).
 
 Axiom dom_unreachable: forall (f:fdef)
+  (Hbinf: branchs_in_fdef f) 
   (Hhasentry: getEntryBlock f <> None)
   (l3 : l) (l' : l) ps cs tmn
-  (Hsucc: dom_analysis_is_successful f)
   (HuniqF: uniqFdef f)
   (HBinF : blockInFdefB (block_intro l3 ps cs tmn) f = true)
   (Hunreach: ~ reachable f l3),
   dom_query f l3 = bound_fdef f.
-
-Axiom dom_is_sound : forall (f : fdef)
-  (Hhasentry: getEntryBlock f <> None)
-  (l3 : l) (l' : l) ps cs tmn
-  (HBinF : blockInFdefB (block_intro l3 ps cs tmn) f = true)
-  (Hin : In l' (l3::(dom_query f l3))),
-  domination f l' l3.
 
 Axiom pres_dom_query: forall 
   (ftrans: fdef -> fdef) 
@@ -80,17 +77,6 @@ Axiom pres_dom_query: forall
   (f : fdef) (l5 l0 : l),
   ListSet.set_In l5 (dom_query f l0) <->
   ListSet.set_In l5 (dom_query (ftrans f) l0).
-
-Axiom pres_dom_analysis_is_successful : forall 
-  (ftrans: fdef -> fdef) 
-  (btrans: block -> block)
-  (ftrans_spec: forall fh bs, 
-    ftrans (fdef_intro fh bs) = fdef_intro fh (List.map btrans bs))
-  (btrans_eq_label: forall b, getBlockLabel b = getBlockLabel (btrans b))
-  (btrans_eq_tmn: forall b, 
-    terminator_match (getBlockTmn b) (getBlockTmn (btrans b))) f,
-  dom_analysis_is_successful f <-> 
-    dom_analysis_is_successful (ftrans f).
 
 End ALGDOM.
 
@@ -108,6 +94,55 @@ Section sound.
 Variable f : fdef.
 Hypothesis Hhasentry: getEntryBlock f <> None.
 
+Lemma dom_is_sound : forall
+  (l3 : l) (l' : l) ps cs tmn
+  (HBinF : blockInFdefB (block_intro l3 ps cs tmn) f = true)
+  (Hin : In l' (l3::(adom.dom_query f l3))),
+  domination f l' l3.
+Proof.
+  unfold domination. autounfold with cfg.
+  intros. destruct f as [fh bs].
+  remember (getEntryBlock (fdef_intro fh bs)) as R.
+  destruct R; try congruence. clear Hhasentry.
+  destruct b as [l5 ps5 cs5 t5].
+  intros vl al Hreach.
+  generalize dependent ps.
+  generalize dependent cs.
+  generalize dependent tmn.
+  remember (ACfg.vertexes (successors (fdef_intro fh bs))) as Vs.
+  remember (ACfg.arcs (successors (fdef_intro fh bs))) as As.
+  unfold ATree.elt, l in *.
+  remember (index l3) as v0.
+  remember (index l5) as v1.
+  generalize dependent bs.
+  generalize dependent l3.
+  generalize dependent l5.
+  induction Hreach; intros; subst.
+    inv Heqv0. symmetry in HeqR.
+    apply adom.dom_entrypoint in HeqR.
+    rewrite HeqR in Hin.
+    simpl in Hin. destruct Hin as [Hin | Hin]; tinv Hin; auto.
+
+    destruct y as [a0].
+    assert (exists ps0, exists cs0, exists tmn0,
+      blockInFdefB (block_intro a0 ps0 cs0 tmn0) (fdef_intro fh bs) /\
+      In l3 (successors_terminator tmn0)) as J.
+      eapply successors__blockInFdefB; eauto.
+    destruct J as [ps0 [cs0 [tmn0 [HBinF'' Hinsucc]]]].
+    destruct (id_dec l' l3); subst; auto.
+    left.
+    assert (In l'
+      (a0 :: (adom.dom_query (fdef_intro fh bs) a0))) as J.
+      assert (incl (adom.dom_query (fdef_intro fh bs) l3)
+                   (a0 :: (adom.dom_query (fdef_intro fh bs) a0))) as Hinc.
+        eapply adom.dom_successors; eauto.
+      simpl in Hin. destruct Hin; try congruence.
+      apply Hinc; auto.
+    eapply IHHreach in J; eauto.
+    simpl.
+    destruct J as [J | J]; subst; eauto.
+Qed.
+
 Lemma sdom_is_sound : forall
   (l3 : l) (l' : l) ps cs tmn
   (HBinF : blockInFdefB (block_intro l3 ps cs tmn) f = true)
@@ -115,7 +150,7 @@ Lemma sdom_is_sound : forall
   strict_domination f l' l3.
 Proof. 
   intros.
-  eapply adom.dom_is_sound with (l':=l') in HBinF; simpl; eauto.
+  eapply dom_is_sound with (l':=l') in HBinF; simpl; eauto.
   unfold strict_domination, domination in *.
   remember (getEntryBlock f) as R.
   destruct R; try congruence.
@@ -144,7 +179,7 @@ Proof.
           destruct f. eapply adom.dom_successors; eauto.
         simpl in Hin.
         apply Hinc; auto.
-      eapply adom.dom_is_sound in J; try solve [eauto 1 | congruence].
+      eapply dom_is_sound in J; try solve [eauto 1 | congruence].
       unfold domination in J.
       rewrite <- HeqR in J.
       assert (Hw:=H).
@@ -187,7 +222,7 @@ Definition getEntryBlock_inv f := forall
   (H : getEntryBlock f = Some (block_intro a ps0 cs0 tmn0)),
   l' <> a.
 
-Lemma adom_acyclic: forall f
+Lemma sdom_acyclic: forall f
   (HgetEntryBlock_inv : getEntryBlock_inv f)
   l1 l2 ps1 cs1 tmn1 ps2 cs2 tmn2,
   reachable f l2 ->
@@ -216,7 +251,6 @@ Include Type ALGDOM.
 Parameter create_dom_tree : fdef -> option (@DTree l).
 
 Axiom dtree_edge_iff_idom: forall (f:fdef)
-  (Hok: dom_analysis_is_successful f)
   (dt: @DTree l)
   (Hcreate: create_dom_tree f = Some dt)
   (le:l) (Hentry: getEntryLabel f = Some le)
@@ -224,13 +258,13 @@ Axiom dtree_edge_iff_idom: forall (f:fdef)
   (Hwfcfg: forall (p : l) (ps0 : phinodes) (cs0 : cmds) 
                   (tmn0 : terminator) (l2 : l),
            blockInFdefB (block_intro p ps0 cs0 tmn0) f ->
-           In l2 (successors_terminator tmn0) -> In l2 (bound_fdef f)),
+           In l2 (successors_terminator tmn0) -> In l2 (bound_fdef f))
+  (Huniq: uniqFdef f),
   forall p0 ch0,
     is_dtree_edge eq_atom_dec dt p0 ch0 = true <-> 
       (imm_domination f p0 ch0 /\ reachable f ch0).
 
 Axiom create_dom_tree__wf_dtree: forall (f:fdef)
-  (Hok: dom_analysis_is_successful f)
   (dt: @DTree l)
   (Hcreate: create_dom_tree f = Some dt)
   (le:l) (Hentry: getEntryLabel f = Some le)
@@ -238,7 +272,8 @@ Axiom create_dom_tree__wf_dtree: forall (f:fdef)
   (Hwfcfg: forall (p : l) (ps0 : phinodes) (cs0 : cmds) 
                   (tmn0 : terminator) (l2 : l),
            blockInFdefB (block_intro p ps0 cs0 tmn0) f ->
-           In l2 (successors_terminator tmn0) -> In l2 (bound_fdef f)),
+           In l2 (successors_terminator tmn0) -> In l2 (bound_fdef f))
+  (Huniq: uniqFdef f),
   ADProps.wf_dtree (successors f) le eq_atom_dec dt.
 
 End ALGDOM_WITH_TREE.
